feat: complete id_correct_implicit and progress on main proof
-Added context to translate_term
-An incorrect translation now generates an Error term which is used to get rid of invalid terms (not semantically correct but a decent workaround)
- Main proof is almost complete, I still need to figure out what to do if the final term is a free variable (is this a value? or an incorrect term?) and have to create a lemma for Apply or generate all cases explicitly

theories/PIR.v
@@ -116,6 +116,7 @@ Inductive term :=
   | Apply    : term -> term -> term
   | Builtin  : DefaultFun -> term
   | Constant : constant -> term
+  | Error    : ty -> term
 .
 
 Declare Scope plutus_scope.
