theories/Semantics.v
@@ -9,31 +9,105 @@ From VTL Require Import PIR BigStepPIR Translation.
 
 Existing Instance EWcbvEval.default_wcbv_flags.
 
+Definition InSubset gt :=
+  match gt with
+  | tRel _
+  | tLambda _ _
+  | tApp (tLambda _ _) _ => True
+(* | some primitive value to replace vars with *)
+  | _ => False
+  end.
+
 Definition gal_id :=
-  tLambda (BasicAst.nNamed "x") (tVar "x").
+  tLambda (BasicAst.nNamed "x") (tRel 0).
+
+Import Coq.Strings.String.
+Local Open Scope string_scope.
+
+Ltac solve_pir_eval := split; [(eexists ; eauto using eval) | constructor].
+Ltac solve_err := simpl in *; contradiction.
 
 Lemma galEvalId : forall Σ, Σ e⊢ gal_id ⇓ gal_id.
 Proof.
   intros. eauto.
 Qed.
 
-Theorem id_correct : forall Σ, Σ e⊢ gal_id ⇓ gal_id ->
-  ((translate_term remap_env gal_id) ann_id) ⇓ ((translate_term remap_env gal_id) ann_id).
+Theorem id_correct_explicit : forall Σ, Σ e⊢ gal_id ⇓ gal_id ->
+  let gal_id' := (translate_term remap_env nil gal_id
+    (TArr (TConst <%% unit %%>) (TConst <%% unit %%>), (TConst <%% unit %%>))) in
+  gal_id' ⇓ gal_id'.
 Proof with (eauto using eval).
   intros.
-  unfold gal_id in *.
-  simpl in *. split.
-  - eexists...
-  - constructor.
+  unfold gal_id' in *.
+  simpl in *. split... constructor.
+Qed.
+
+Theorem id_correct_implicit : forall Σ ctx (ann : annots box_type gal_id),
+  let gal_id' := translate_term remap_env ctx gal_id ann in
+  Σ e⊢ gal_id ⇓ gal_id ->
+  InSubset gal_id ->
+  ~ (isError gal_id') ->
+  gal_id' ⇓ gal_id'.
+Proof with (eauto using eval).
+  intros. simpl in gal_id'.
+  destruct ann eqn:Ea. destruct (decompose_arr b).
+  destruct l; try solve_err; 
+  unfold get_type in gal_id';
+  try solve_pir_eval;
+  try solve_err.
+  induction b1;
+  try solve_pir_eval;
+  try solve_err.
+  destruct (Env.with_default (UNDEFINED "NotInMap")
+  (Env.lookup remap_env
+  (bs_to_s Kernames.string_of_kername k)));
+  try solve_pir_eval;
+  try solve_err.
+Qed.
+
+Theorem trans_lambda : forall ctx na t bt1 bt2 (ann : annots box_type t),
+  let lt := translate_term remap_env ctx (tLambda na t) (TArr bt1 bt2, ann) in
+  ~ (isError lt) ->
+  lt ⇓ lt.
+Proof with (eauto using eval).
+  intros.
+  simpl in lt. destruct (decompose_arr bt2).
+  - induction bt1; unfold get_type in lt;
+  try solve_pir_eval;
+  try solve_err.
+  (* this is fragile*)
+  destruct (Env.with_default (UNDEFINED "NotInMap")
+  (Env.lookup remap_env
+  (bs_to_s Kernames.string_of_kername k)));
+  try solve_pir_eval;
+  try solve_err.
 Qed.
 
 Theorem translation_correct : 
-  forall Σ gt (ann : annots box_type gt),
+  forall Σ ctx gt (ann : annots box_type gt),
+  let gt' := translate_term remap_env ctx gt ann in
   Σ e⊢ gt ⇓ gt ->
-  (* InSubset gt -> *)
-  (translate_term remap_env gt ann) ⇓ (translate_term remap_env gt ann).
-Proof.
-  intros.
-  induction H.
-  (* discriminate using InSubset gt *)
+  InSubset gt ->
+  ~ isError gt' ->
+  gt' ⇓ gt'.
+Proof with (eauto using eval).
+  intros Σ ctx gt ann gt' ev sub nerr. 
+  destruct gt eqn:Egt; simpl in gt';
+  (* this gets rid of terms that are not implemented or give a trivial error *)
+  try solve_err.
+  (* - (* tBox => Constant, add this if tBox is in the subset *) try solve_pir_eval. *)
+  - (* tRel *) destruct (nth_error ctx n).
+    + destruct c. destruct decl_name.
+      * solve_err.
+      * split.
+        ** eexists. unfold gt'. admit. (* what to do in var case *)
+        ** unfold gt'. admit.
+    + solve_err.
+  - (* tLambda *) destruct ann eqn:Ea. destruct b; simpl in gt';
+    try solve_err.
+    + apply trans_lambda. simpl. destruct (decompose_arr b2).
+      destruct (get_type remap_env b1)...
+  - (*tApp*) destruct t1; simpl in sub; try contradiction.
+    (* lemma that is valid for all types that make sense *)
+    simpl in *. admit.
 Admitted.
