theories/Translation.v
@@ -5,7 +5,7 @@ From MetaCoq.Erasure.Typed Require Import TypeAnnotations.
 From MetaCoq.Erasure.Typed Require Import Extraction.
 From MetaCoq.Erasure.Typed Require Import ResultMonad.
 From MetaCoq.Erasure Require Import EAst EAstUtils.
-From MetaCoq.Utils Require Import MCList MCPrelude.
+From MetaCoq.Utils Require Import MCList MCString MCPrelude.
 
 From VTL Require Import Env PIR.
 
@@ -45,41 +45,61 @@ Definition get_name (na : name) : string :=
 
 Definition get_type (TT : env PIR.ty) : box_type -> PIR.ty :=
   fix go (bt : box_type) :=
-match bt with
-| TBox => PIR.Ty_Builtin (PIR.DefaultUniUnit)
-| TArr dom codom => PIR.Ty_Fun (go dom) (go codom)
-| TConst kn => let cst := string_of_kername kn in
-    with_default (PIR.UNDEFINED "NotInMap") (lookup TT cst)
-| TAny => PIR.UNDEFINED "UnknownType"
-| _ => PIR.UNDEFINED "NotImplemented"
-end.
+  match bt with
+  | TBox => PIR.Ty_Builtin (PIR.DefaultUniUnit)
+  | TArr dom codom => PIR.Ty_Fun (go dom) (go codom)
+  | TConst kn => let cst := string_of_kername kn in
+      with_default (PIR.UNDEFINED "NotInMap") (lookup TT cst)
+  | TAny => PIR.UNDEFINED "UnknownType"
+  | _ => PIR.UNDEFINED "NotImplemented"
+  end.
 
 (* translation based on ConCerts cameLIGO extraction *)
-Fixpoint translate_term (TT : env PIR.ty) (t : term) 
+Fixpoint translate_term (TT : env PIR.ty) (ctx : context) (t : term) 
                         {struct t} : annots box_type t -> PIR.term :=
-match t return annots box_type t -> PIR.term with
-| tVar n => fun bt => PIR.Var n
-| tLambda na body => fun '(bt, a) =>
-  let na' := get_name na in (* get fresh name from context? *)
-  let (dom_tys, _) := ExAst.decompose_arr bt in
-  let dom_ty := match nth_error dom_tys 0 with
-                | Some ty => get_type TT ty
-                | None => PIR.UNDEFINED "TypeNotInDomain"
-                end in
-      PIR.LamAbs na' dom_ty (translate_term TT body a) (* extend context *)
-| tApp t1 t2 => fun '(bt, (T1, T2)) => 
-    PIR.Apply (translate_term TT t1 T1) (translate_term TT t2 T2) (* fails for multiple arguments *)
-| _ => fun _ => PIR.Var "notSupported"
-end.
+  match t return annots box_type t -> PIR.term with
+  | tBox => fun bt => PIR.Constant (ValueOf DefaultUniUnit tt) (* boxes become the constructor of the [unit] type *)
+  | tRel n => fun bt =>
+    match nth_error ctx n with
+    | Some {| decl_name := na |} =>
+      match na with
+      | nAnon => PIR.Error (PIR.UNDEFINED ("Anonymous (" ++ string_of_nat n ++ ")"))
+      | nNamed id => PIR.Var id
+      end
+    | None => PIR.Error (PIR.UNDEFINED ("UnboundRel(" ++ string_of_nat n ++ ")"))
+    end
+  | tLambda na body => fun '(bt, a) =>
+      match ExAst.decompose_arr bt with
+      | ([], _) => PIR.Error (PIR.UNDEFINED "LambdaTypeIsNotAFunction")
+      | (ty :: _, _) =>
+        match get_type TT ty with
+        | PIR.UNDEFINED _ => PIR.Error (PIR.UNDEFINED "TypeNotDefined")
+        | ty' => let na' := get_name na in (* get fresh name from context *)
+          LamAbs na' ty' (translate_term TT (vass (nNamed (s_to_bs na')) :: ctx) body a) 
+        end
+      end
+  | tApp t1 t2 => fun '(bt, (T1, T2)) => 
+      PIR.Apply (translate_term TT ctx t1 T1) (translate_term TT ctx t2 T2) (* fails for multiple arguments *)
+  | _ => fun _ => PIR.Error (PIR.UNDEFINED "NotSupported")
+  end.
+
+(* When the translation becomes more complicated, we might need to recurse *)
+Fixpoint isError pt : Prop :=
+  match pt with
+  | PIR.Error _ => True
+  | PIR.LamAbs _ _ b => isError b
+  | PIR.Apply pt1 pt2 => isError pt1 /\ isError pt2 
+  | _ => False
+  end.
 
 (* Lambda Box T is the combination of an EAst term with a dependent tree of its types
   For now, we pass manual annotations until I set up a proper pipeline *)
 
 Definition identity_EAst : term :=
-  tLambda (nNamed (s_to_bs "x")) 
-    (tVar (s_to_bs "x")).
+  tLambda (nNamed (s_to_bs "y")) 
+    (tRel 0).
 
 Definition ann_id :=
   (TArr (TConst <%% Z %%>) (TConst <%% Z %%>), (TConst <%% Z %%>)).
 
-Eval cbv in (translate_term remap_env identity_EAst ann_id).
+Eval cbv in (translate_term remap_env nil identity_EAst ann_id).
