theories/Printer.v
@@ -28,7 +28,7 @@ RunIO IOMode Forward.
 (* Automatically assign the right integer types (hopefully) *)
 RunIO Smart On.
 
-Definition test_pir_ast := ((translate_term remap_env identity_EAst) ann_id).
+Definition test_pir_ast := ((translate_term remap_env nil identity_EAst) ann_id).
 Eval cbv in (print_as_program test_pir_ast).
 Definition main : IO unit :=
   chan <- open_out "./output/test.pir" ;;
